Make files type-check

compilerProofScript.sml
@@ -1,6 +1,6 @@
 Theory compilerProof
 Ancestors
-  panLang panProps panSem compiler p4 p4_bigstep p4_exec_sem
+  panLang panProps panSem compiler p4 p4_full_bigstep p4_exec_sem p4_ebpf
 Libs
   wordsLib
 
@@ -11,7 +11,7 @@ Type scope = ``:((varn, (v # lval option)) alist)``;
 Type state = 
     <| locals      : varname |-> 'a v
      ; globals     : varname |-> 'a v
-e     ; code        : funname |-> ((varname # shape) list # ('a panLang$prog))
+     ; code        : funname |-> ((varname # shape) list # ('a panLang$prog))
                      (* arguments (with shape), body *)
      ; eshapes     : eid |-> shape
      ; memory      : 'a word -> 'a word_lab
@@ -26,30 +26,37 @@ e     ; code        : funname |-> ((varname # shape) list # ('a panLang$prog))
 val s = ``(s:('a,'ffi) panSem$state)``
 *)
 
+
+        
 (*----VERIFICATIONS----*)
   
 (* Semantic properties of the value-relations *)
 Inductive v_rel:
   v_rel (e_v (v_bool T)) (Val (Word 1w)) ∧
   v_rel (e_v (v_bool F)) (Val (Word 0w)) ∧
-  (v_rel (e_v (v_bit (b,l))) (Val (Word wrd)) ∧ MAP (\(x,y).case (x,y) of (T,1) => T | (F,0) => T | (_,_) => F) $ ZIP (b,word_to_bin_list (wrd:word64)))
+  (*(v_rel (e_v (v_bit (b,l))) (Val (Word wrd)) && MAP (\(x,y).case (x,y) of (T,1) => T | (F,0) => T | (_,_) => F) $ ZIP (b,word_to_bin_list (wrd:word64)))*)
+  (*(v_rel (e_v (v_str s)) (Struct vals) && EVERY (\((wrd1, _), Val Word wrd2). case (word_compare wrd1 wrd2) of 1w => T | 0w => F) $ ZIP ((REPLICATE 8 chars_to_word (string_to_chars s)), vals))*)
+End
+
+Inductive state_rel:
+  s_rel 
 End
 
 Theorem compile_exp_correct:
-  (∀ e uninit (scope_lists:scope_list) e' (n:num) m pan_e s.
+  (∀ e uninit (scope_lists:scope_list) e' (n:num) m env pan_e s.
     bigstep_e_exec uninit (scope_lists:scope_list) (INL (e)) (n:num) = SOME $ (INL e', m) ∧
-    is_v e' ∧ compile_exp e = SOME pan_e ∧ state_rel scope_lists s ⇒
+    is_v e' ∧ compile_exp env e = SOME (env, pan_e) ∧ state_rel scope_lists s ⇒
     ∃ v. eval s pan_e = SOME v ∧
          v_rel e' v ) ∧
-  ∀ es uninit (scope_lists:scope_list) es' (n:num) m pan_es s.
+  ∀ es uninit (scope_lists:scope_list) es' (n:num) m env pan_e s.
     bigstep_e_exec uninit (scope_lists:scope_list) (INR (es)) (n:num) = SOME $ (INR es', m) ∧
-    EVERY is_v es' ∧ OPT_MMAP compile_exp es = SOME pan_es ∧ state_rel scope_lists s ⇒
+    EVERY is_v es' ∧ EVERY (\x. compile_exp env x = SOME (env, pan_e)) es ∧ state_rel scope_lists s ⇒
     ∃ vs. OPT_MMAP (eval s) pan_es = SOME vs ∧
          LIST_REL v_rel es' vs                     
 Proof
   Induct
   >~ [‘e_v _’]
-  >- (rw [compile_exp_def, bigstep_e_exec_def, AllCaseEqs()] >> rw [eval_def] >> metis_tac [v_rel_rules])
+  >- Cases_on ‘n’ >> (rw [compile_exp_def, bigstep_e_exec_def, AllCaseEqs()] >> (rw [eval_def] >> metis_tac [v_rel_rules]))
   >~ [‘e_unop _’]
   >- (rw [compile_unop_def, compile_exp_def, bigstep_e_exec_def, AllCaseEqs()]
   >- (gvs[oneline e_exec_unop_def, AllCaseEqs(), oneline unop_exec_def] >> first_x_assum drule_all >> strip_tac >> rw[eval_def] >> gvs[v_rel_cases] >> gvs[wordLangTheory.word_op_def] >> gvs[wordLangTheory.word_op_def])
@@ -62,7 +69,7 @@ Proof
   >- cheat)
   >~ [‘e_binop _’]
   >- cheat
-  >~ [‘e_var _’]
+  >~ [‘e_var _’] 
   >- cheat
   >~ [‘e_acc _ _’]
   >- cheat
@@ -85,3 +92,14 @@ Proof
   >~ [‘INR (_::_)’]
   >- cheat >> gvs [compile_exp_def]
 QED
+
+
+        
+(*
+REDO 
+Theorem compile_stmt_correct:
+
+Proof
+
+QED
+*)
