compilerScript.sml
@@ -3,6 +3,7 @@ Ancestors
   panLang
   p4
   finite_map
+  p4_ebpf
           
 val _ = monadsyntax.temp_add_monadsyntax()
 val _ = monadsyntax.enable_monad "option"
@@ -13,10 +14,12 @@ val _ = monadsyntax.enable_monad "option"
 Type state_dict  = “:varname |-> ('a prog list)” (* To create stmts for the state-machine if-elses *)
 Type scope_dict  = “:varname |-> varkind”        (* Global or Local, for funn and varnn *)
 Type staten_dict = “:64 exp |-> word64”
-Type out_ind_dict = “:varname |-> num list” (* Function to parameter position *)
+Type out_ind_dict = “:varname |-> num list”      (* Name to parameter position *)
+Type out_val_dict = “:64 panLang$exp |-> num list”
+Type apply_table = “:ebpf_ctrl”
 
 Datatype:
-  env_rec = <| states : 'a ; scopes : 'b; state_nums : 'c ; out_ind : 'd ; table : e' |>
+  env_rec = <| states : 'a ; scopes : 'b; state_nums : 'c ; out_s_ind_pairs : 'd ; table : 'e ; ass_var : 'f ; out_ind_val_pairs : 'g ; match_fun : 'h|>
 End
       
 Definition lLEFT_def:
@@ -27,6 +30,10 @@ Definition lRIGHT_def:
   lRIGHT l = MAP (\(l,r).r) l
 End
 
+Definition lCOPY_def:
+  lCOPY l = FOLDR (\e t. e::t) [] l
+End
+
 (* TODO *)
 Definition lval_to_mlstring_def:
   lval_to_mlstring (lval_varname varname)   = strlit "TEMP-VARNAME" ∧
@@ -34,6 +41,15 @@ Definition lval_to_mlstring_def:
   lval_to_mlstring (lval_field lval s)      = strlit "TEMP-FIELD-to_mlstring not finished" ∧
   lval_to_mlstring (lval_slice lval e1 e2)  = strlit "TEMP-SLICE-to_mlstring not finished" ∧
   lval_to_mlstring (lval_paren lval)        = strlit "TEMP-PAREN-to_mlstring not finished"
+End
+
+(* TODO *)
+Definition lval_to_string_def:
+  lval_to_string (lval_varname varname)   = "TEMP-VARNAME" ∧
+  lval_to_string (lval_null)              = "TEMP-NULL--to_string not finished" ∧
+  lval_to_string (lval_field lval s)      = "TEMP-FIELD-to_string not finished" ∧
+  lval_to_string (lval_slice lval e1 e2)  = "TEMP-SLICE-to_string not finished" ∧
+  lval_to_string (lval_paren lval)        = "TEMP-PAREN-to_string not finished"
 End
 
 (* TODO *)
@@ -59,45 +75,113 @@ End
 
 Definition string_to_struct_def:
   string_to_struct s =
-  do
-     cs <<- string_to_chars s;
-     wrds_pair <<- REPLICATE 8 (chars_to_word cs);
-     pan_wrds <<- MAP (\w.Const w) $ lLEFT wrds_pair;
-     Struct $ pan_wrds
-  od
+  (let
+     cs = string_to_chars s;
+     wrds_pair = REPLICATE 8 (chars_to_word cs);
+     pan_wrds  = MAP (\w.Const w) $ lLEFT wrds_pair;
+   in
+     Struct $ pan_wrds)
+End
+
+Definition bit_v_to_word_def:
+  bit_v_to_word bools n =
+  (let
+     wrd_indx_list = ZIP ((MAP (\b.case b of T => 1w :word64 | F => 0w :word64) bools), (GENLIST (\m.m) n));
+     wrd = FOLDR (\(m,i) c.(m << i) ⊕ c) (0w :word64) wrd_indx_list;
+   in
+        wrd :64 word)
+End
+
+(*TODO: all these functions---make unique and properly functioning*)
+Definition get_trans_name:
+  get_trans_name = strlit "trans"
 End
 
 Definition get_fun_name_def:
-  get_fun_name s = NONE
+  get_fun_name s = "fun"
 End
 
 Definition get_var_name_def:
-  get_var_name s = NONE
+  get_var_name s = "var"
 End
 
-Definition to_no_name_def:
-  to_no_name = strlit ""
+Definition get_match_fun_name_def:
+  get_match_fun_name = strlit "match_fun"
+End
+        
+Definition get_no_name_def:
+  get_no_name = strlit ""
 End
 
 (* Generates a new, unique (to this compiler!) variable_name *)
 (* TODO: to implement a true unique name-generator we need to rename all variable also *)
 Definition generate_varname_def:
-  generate_varname = NONE
+  generate_varname env = (env, strlit "")
 End
 
 (* Generates a list of Varnames, all unique. Empty list results in 'no name' and, thus, returns an empty list. *)
 (* TODO: to implement a true unique name-generator we need to rename all variable also *)
 Definition generate_varnames_def:
-  generate_varname [] = []
-  generate_varnames l = NONE
+  generate_varnames env l = (env, strlit "")
 End
+
+Definition FOLDM_def:
+  FOLDM fun a [] = return a ∧
+  FOLDM fun a (b::bs) =
+  do
+    a' <- fun a b;
+    FOLDM fun a' bs
+  od
+End
+
+Theorem FOLDM_CONG[defncong]:
+  !l l' b b' (f: 'a->'b->'a option) f'.
+    l=l' /\ b=b' /\ (!x a. MEM x l' ==> (f a x = f' a x))
+          ==>
+    FOLDM f b l = FOLDM f' b' l'
+Proof
+cheat
+  (*Induct
+  THEN REWRITE_TAC [FOLDR, MEM]
+  THEN REPEAT STRIP_TAC
+  THEN REPEAT (PAT_X_ASSUM (Term‘x = y’) (SUBST_ALL_TAC o SYM))
+  THEN REWRITE_TAC [FOLDR]
+  THEN POP_ASSUM (fn th => MP_TAC (SPEC (Term‘h’) th) THEN ASSUME_TAC th)
+  THEN REWRITE_TAC [MEM]
+  THEN DISCH_TAC
+  THEN MK_COMB_TAC
+  THENL [CONV_TAC FUN_EQ_CONV THEN ASM_REWRITE_TAC [],
+         FIRST_ASSUM MATCH_MP_TAC THEN ASM_REWRITE_TAC []
+           THEN REPEAT STRIP_TAC
+           THEN FIRST_ASSUM MATCH_MP_TAC
+           THEN ASM_REWRITE_TAC [MEM]]*)
+QED
+        
+Definition mlstring_EQ_def:
+  mlstring_EQ s1 s2 = T
+End
+
+                
 (*-------------------------------------------------*)
-(*                  COMPILER                       *)
+(*                 eBPF FUNCTIONS                  *)
+(*-------------------------------------------------*)
+(*
+TODO:   - finish
+        - make dynamic for architecture used.
+*)
+Definition match_fun_def:
+  match_fun v s = s
+End
+        
+(*-------------------------------------------------*)
+(*                    COMPILER                     *)
 (*-------------------------------------------------*)
 (*
 Assumes that Pancake deals with overflowing values (for the saturated ADD and SUB).
         
 Paramethers: op : unop in P4, pan_eX is a (compiled P4) Pancake expression
+
+             TODO: fix faulty binpos: lisst cons!
 *)
 Definition compile_binop_def:
   compile_binop (pan_e1, op, pan_e2) = case op of
@@ -142,53 +226,51 @@ Definition compile_unop_def:
   | unop_neg_signed => Op Add [Op Xor [pan_e; Const(0xFFFFFFFFFFFFFFFFw:word64)]; Const(0xFFFFFFFFFFFFFFFFw:word64)]               
   | unop_un_plus    => Op Add [pan_e; Const(0w:word64)]
 End
-        
+
+(* TODO: termination for the FOLM (lambda) in e_call *)
 Definition compile_exp_def:
   compile_exp env (e_binop e1 op e2)  =
   do
-    (env', e1') <- compile_exp env e1;
-    (env', e2') <- compile_exp env e2;
-    return (env', compile_binop (e1', op, e2'))
+    (env',  stmts1, e1') <- compile_exp env e1;
+    (env'', stmts2, e2') <- compile_exp env' e2;
+    return (env'', stmts1++stmts2, compile_binop (e1', op, e2'))
   od                                     ∧       
   compile_exp env (e_unop op e)       =                     (* unop is only called on e=bool or bitv *)
   do
-    (env', e') <- compile_exp env e;
-    return (env', compile_unop (op, e'))
+    (env', stmts, e') <- compile_exp env e;
+    return (env', stmts , compile_unop (op, e'))
   od                                     ∧
   compile_exp env (e_call funn es)    =
   do
     case env.ass_var of
-      strlit "" =>
+      varn_name "" => NONE
+    | varn_name x =>
         do
-          (* TODO: do normal call *)
-        od
-    | var_name  =>
-        do
-          function_name <- get_fun_name funn;
-          args_pan      <- compile_exp es
-          out_iv_pair   <- env.out_ind_value_pairs function_name;
-          out_vars      <- OPT_MMAP ((\as i. get_element i as) args_pan) (lLEFT out_iv_pair);
+          function_name <<- strlit $ get_fun_name funn;
+          (env', sl, args_pan) <- FOLDM (\(e, sl, l) x. do (e', sl', x') <- compile_exp e x; return (e', sl++sl', l++[x']) od) (env, [], []) es;
+          out_iv_pairs  <<- ([] : (num # 64 panLang$exp) list); (*(env'.out_ind_value_pairs) function_name;*)
+          out_vars      <<- MAP (\i. EL i args_pan) (lLEFT out_iv_pairs);
           out_var_names <- OPT_MMAP (\e. case e of (Var v_kind v_name) => SOME v_name | _ => NONE) out_vars;
-          s1   <<- DecCall var_name One function_name (OPT_MMAP args_pan) Skip;                                          (* TODO: deal with shape! *)
-          s2   <<- FOLDL (\s (name, v). Seq (Assign Local name v) s) Skip ZIP (out_vnms, (lRIGHT out_iv_pair));
-          env' <<- env with ass_var := get_no_name;
-          return (env', Seq s1 s2)
+          varname <<- strlit (get_var_name x);
+          s1   <<- DecCall varname One function_name args_pan Skip; 
+          s2   <<- FOLDL (\s (name, v). Seq (Assign Local name v) s) Skip $ ZIP (out_var_names, (lRIGHT out_iv_pairs));
+          env'' <<- env' with ass_var := varn_name "";
+          return (env'', sl++[Seq s1 s2], Var Local varname)
         od
   od ∧
   compile_exp env (e_list es)         = NONE ∧             
   compile_exp env (e_var varn)        = (case varn of      (* TODO: need lookup! *)
-    varn_name n  => return $ (env, Var Local (strlit n))
+    varn_name n  => return $ (env, [] , Var Local (strlit n))
   | varn_star fn => NONE)                   ∧            
   compile_exp env (e_v val)           = (case val of
-    v_bool T        => return $ (env, Const(1w:word64))
-  | v_bool F        => return $ (env, Const(0w:word64))
-  | v_bit (bools,n) =>
+    v_bool T        => return $ (env, [], Const(1w:word64))
+  | v_bool F        => return $ (env, [], Const(0w:word64))
+  | v_bit (bools,n) => (*TODO: bit-arrays longer than 64 bits*)
       (let
-         wrd_indx_list = ZIP ((MAP (\b.case b of T => 1w :word64 | F => 0w :word64) bools), (GENLIST (\m.m) n));
-         wrd = FOLDR (\(m,i) c.(m << i) ⊕ c) (0w :word64) wrd_indx_list;
+         wrd = bit_v_to_word bools n
        in
-         return $ (env, Const wrd))
-  | v_str s         => return (env, string_to_struct s)
+         return $ (env, [], Const wrd))
+  | v_str s         => return (env, [], string_to_struct s)
   | v_struct svs    => NONE
   | v_header b svs  => NONE
   | v_ext_ref i     => NONE
@@ -203,7 +285,20 @@ Definition compile_exp_def:
   compile_exp _ _ = NONE
 End
 
-        
+Definition compile_exps_def:
+  compile_exps env [] = return (env, [], []) ∧
+  compile_exps env (e::es) =
+  do
+    (env',  stmts1, e_pan)  <- compile_exp env e;
+    (env'', stmts2, e_pans) <- compile_exps env' es;
+    return (env'', stmts1++stmts2, e_pan::e_pans)
+  od
+End
+
+Definition compile_set_exp_def:
+  compile_set_exp env es = compile_exps env es
+End
+
 (* TODO
    - input enviroment/enviroment entvienment
    - variables need env-table check for varkind value
@@ -214,34 +309,38 @@ Definition compile_stmt_def:
   compile_stmt env (stmt_ass lval e)           =
   (case env.out_s_ind_pairs of
      [] =>
-      do
-        env' <- env with ass_var := lval_to_mlstring lval;
-        (env'', e') <- compile_exp env' e;
-        env''' <- env'' with ass_var := strlit "";
-        return (env''', Assign Local (lval_to_mlstring lval) (e'))
+       do
+        (*--IN ASS. STMT---*)
+        env' <<- env with ass_var := varn_name $ get_var_name $ lval_to_string lval;
+        (env'', stmts, e') <- compile_exp env' e;
+        env''' <<- env'' with ass_var := varn_name "";
+        (*-----------------*)
+        return (env''', FOLDR Seq (Assign Local (strlit (get_var_name (lval_to_string lval))) (e')) stmts)
       od 
    | pairs  =>
-      do
-        name <- get_var_name lval;
-        env' <<- env with ass_var := name;
-        (env'', e_pan) <- compile_exp env' e;
-        env''' <<- env'' with ass_var := strlit "";
-        ind <- FOLDL ((\n i (s, ind). if ((get_var_name s) == n) then (SOME i) else NONE) name) (SOME 0) pairs;
+       do
+        (*--IN ASS. STMT---*)
+        name <<- get_var_name $ lval_to_string lval;
+        env' <<- env with ass_var := varn_name name;
+        (env'', stmts, e_pan) <- compile_exp env' e;
+        env''' <<- env'' with ass_var := varn_name "";
+        (*-----------------*)
+        ind <- FOLDL (\ i (s, ind). if (mlstring_EQ (get_var_name s) (strlit name)) then (SOME ind) else i) NONE pairs;
         env4 <<- env''' with out_ind_val_pairs := env'''.out_ind_val_pairs |+ (ind, e_pan);
-        return (env''', Assign Local (name) (e_pan))
+        return (env''', FOLDR Seq (Assign Local (strlit name) (e_pan)) stmts)
       od ) ∧
   compile_stmt env (stmt_cond e stmt_t stmt_f) =
   do
-    (env', e')    <- compile_exp env e;
+    (env', stmts, e')    <- compile_exp env e;
     (env'', pt')  <- compile_stmt env' stmt_t;
     (env''', pf') <- compile_stmt env' stmt_f;
-    return (env', If e' pt' pf')
+    return (env', FOLDR Seq (If e' pt' pf') stmts)
   od                                              ∧
   compile_stmt env (stmt_block t_scope stmt)   = NONE ∧    
   compile_stmt env (stmt_ret e)                =
   do
-    (env', e') <- (compile_exp env e);
-    return (env', Return e')
+    (env', stmts, e') <- (compile_exp env e);
+    return (env', FOLDR Seq (Return e') stmts)
   od                                              ∧
   compile_stmt env (stmt_seq stmt1 stmt2)      =
   do
@@ -251,18 +350,23 @@ Definition compile_stmt_def:
   od                                              ∧
   compile_stmt env (stmt_trans e)              =
   do
-    (env', pan_e) <- (compile_exp env e);
+    (env', stmts, pan_e) <- (compile_exp env e);
     wrd <- FLOOKUP env.state_nums pan_e;
-    return (env', Seq (Assign Local (strlit "trans") (Const wrd)) Break)    
+    return (env', FOLDR Seq (Seq (Assign Local get_trans_name (Const wrd)) Break) stmts)    
   od ∧
   compile_stmt env (stmt_app x es)             = NONE ∧
   compile_stmt env (stmt_ext)                  = NONE ∧
   compile_stmt _ _ = NONE                  
 End
 
+
+Definition to_seq_def:
+  to_seq [] = Skip ∧
+  to_seq (s::ss) = Seq s (to_seq ss)
+End
  
 (*-------------------------------------------------
-Does:
+DOES:
     - Updates enviroment giving every state in block an unique number
     - Compiles each states' stmts
     - Puts those stmts into panLang conditionals (one for each state) with comp. of "trans"-variable and unique number as guard
@@ -278,18 +382,18 @@ Definition compile_states_def:
     (env', _, nums) <<- FOLDL (\(e,i,l) (st_name,_). (env with state_nums := (env.state_nums |+ (string_to_struct st_name, i)), i + (1w :word64), i::l) ) (env, (2w :word64), []) states;
     l <- OPT_MMAP (compile_stmt env') (lRIGHT states);
     (seqs :64 prog list) <<- lRIGHT l;
-    conds <<- FOLDR (\(num, seq) p. If (Cmp Equal (Var Local (strlit "trans")) (Const num)) seq p :64 prog) Skip (ZIP (nums,seqs));
+    conds <<- FOLDR (\(num, seq) p. If (Cmp Equal (Var Local get_trans_name) (Const num)) seq p :64 prog) Skip (ZIP (nums,seqs));
     return (env', conds)
   od
 End
 
 
-(* TODO:
-   - make pr_accept and pr_reject do more than just break
-   - care about specific function call .extract(blah-blah) (puts argument into P4-header structure)  
-*)
+
 (*-------------------------------------------------
 The Parser is a state machine and and is in Pancake translated into a function containing a conditional blocks for every state. Required states are the states: Start, Accept, and Reject.
+
+TODO:   - make pr_accept and pr_reject do more than just break
+        - care about specific function call .extract(blah-blah) (puts argument into P4-header structure)  
 
 Returns: pair of; new enviroment and the panLang prog describing the whole parser
 -------------------------------------------------*)
@@ -299,7 +403,7 @@ Definition compile_parser_def:
      e_trans  = Const (2w:word64); (* start state will always be first in the list of states and so get value 2 *)
      e_accept = Const (1w:word64);
      e_reject = Const (0w:word64);
-     e_var_trans = (Var Local (strlit "trans"):64 exp);
+     e_var_trans = (Var Local get_trans_name:64 exp);
      pr_accept = Break:64 prog;
      pr_reject = Break:64 prog;
    in
@@ -307,7 +411,7 @@ Definition compile_parser_def:
        (env', pr_states) <- compile_states env pars_map;
        pr_if' <<- If ((Cmp Equal) e_var_trans e_reject) pr_reject pr_states;
        pr_if  <<- If ((Cmp Equal) e_var_trans e_accept) pr_accept pr_if';
-       return (env', While (Const (1w:word64)) (Dec (strlit "trans") One e_trans pr_if))
+       return (env', While (Const (1w:word64)) (Dec get_trans_name One e_trans pr_if))
      od)
 End
 
@@ -325,7 +429,18 @@ Definition to_params_def:
   to_params sds = MAP (\(s,d). (s, One)) sds
 End
 
-        
+Definition generate_params_def:
+  generate_params env [] = (env, []) ∧
+  generate_params env (prm::prms) =
+  (let
+     (env', s) = generate_varname env;
+     (env'', ss) = generate_params env' prms
+   in
+     (env'', (s, One)::ss))
+End
+
+
+(*-------------------------------------------------*)        
 (*-------------------------------------------------
 Does: Creates a new function (above the control function block in Pancake) for every control-block local function. Saves index for every "out" or "inout" parameter for that function (as name and num-list pair) in enviroment to be used for copy-out during function calls. Adds all control-block local variables as paramathers to the function.
 
@@ -338,95 +453,134 @@ Definition compile_block_functions_def:
   compile_block_functions env vars [] = return (env, []) ∧
   compile_block_functions env vars ((n, (stmt, ad_list))::b_funcs) =
   do
-    prms <<- (to_params (lLeft ad_list)) ++ vars;
-    out_s_ind_pairs <<- FOLDL (\l ((s, d), ind).  
+    prms <<- (to_params (lLEFT ad_list)) ++ vars;
+    out_sind_pairs <<- FOLDL (\l ((s, d), ind).  
                              case d of
-                               d_out -> (s, ind)::l
-                             | d_inout -> (s, ind)::l
-                             | _ -> l) [] ZIP (ad_list, (GENLIST (\m.m) m));
-    env' <<- env' with out_sinds := out_s_ind_pairs;
+                               d_out => (s, ind)::l
+                             | d_inout => (s, ind)::l
+                             | _ => l) [] $ ZIP (ad_list, (GENLIST (\m.m) (LENGTH ad_list)));
+    env' <<- env with out_s_ind_pairs := out_sind_pairs;
     (env'', b) <- compile_stmt env' stmt;
     decl <<-
-        <|     name   := get_fun_name n
+        <|     name   := strlit (get_fun_name n)
              ; inline := F
              ; export := F
              ; params := prms
              ; body   := b
              ; return := One
         |>;
-    env''' <<- env'' with out_ind_value_pairs := env''.out_ind_value_pairs |+ (get_fun_name n, out_ind_list);
+    (*env''' <<- env'' with out_ind_val_pairs := env''.out_ind_val_pairs |+ (strlit (get_fun_name n), lRIGHT out_sind_pairs);*)
+    env''' <<- env''; (* TODO: *)
     (env4, decls) <- compile_block_functions env''' vars b_funcs;
     return (env4, decl::decls)
   od                               
 End
 
+
+(*-------------------------------------------------
+   DOES: Generates seqence of panLang$prog for matching all parameters to the match_function and ANDs up the result.
+        
+  TAKES: An enviroment, list of exp_pan and list of the apply_tables keys as exp_pan.
+
+RETURNS: An enviroment, AND-variable keeping current AND from all match-results, stmts for searching (possible finding) one action
+-------------------------------------------------*)
 Definition generate_action_matching_def:
-  generate_action_matching env prms =
+  generate_action_matching env [] [] = (env, Var Local (strlit ""), Skip) ∧
+  generate_action_matching env (v_l::[]) (s_l::[]) = (env, Var Local (strlit ""), Skip) ∧ (*TODO*)
+  generate_action_matching env (v_l1::v_ls) (s_l1::s_ls) =
+  (let
+    (env', AND_s : mlstring) = generate_varname env;
+    AND_var       = Var Local AND_s;
+    match_funn    = env'.match_fun : mlstring;
+    stmt          = DecCall AND_s One match_funn (v_l1::[s_l1]) Skip;
+    (env'', prog) = FOLDL (\(e, prev) (v, s). (let (e', RET_s : mlstring) = generate_varname e;
+                                                   RET_var = Var Local RET_s
+                                               in  
+                                                 (e', Seq prev (DecCall RET_s One match_funn (v::[s]) (Assign Local AND_s (Op And ([AND_var]++[RET_var]))))))) (env', stmt) $ ZIP (v_ls, s_ls)
+   in
+     (env'', AND_var, prog))
+End
+
+(*-------------------------------------------------
+ASSUMPTIONS: - priority a bit-vector max 1 word long (n ≤ 64).
+-------------------------------------------------*)
+Definition generate_actions_def:
+  generate_actions env (_,_,_,_) [] = (env, Skip) ∧
+  generate_actions env (prms, a_s, p_s, found) (((s_ls, a_prio), (a, _))::tbls) =
+  (let
+     (env', AND_var, p_a) = generate_action_matching env prms s_ls;
+     cur_prio = Const (bit_v_to_word a_prio (LENGTH a_prio));
+     ass_a    = Assign Local a_s (string_to_struct a);
+     ass_prio = Assign Local p_s cur_prio;
+     prio_var = Var Local p_s;
+     p_false  = Seq ass_a ass_prio;
+     p_true   = If (Cmp Lower prio_var cur_prio) (Seq ass_a ass_prio) Skip;
+     p_true'  = If found p_true p_false;
+     p_false' = Skip;
+     p_conds  = Seq (If AND_var p_true' p_false') (Skip);
+     (env'', prev) = generate_actions env' (prms, a_s, p_s, found) tbls
+   in
+     (env'', Seq (Seq p_a p_conds) prev)) 
+End
+
+(*-------------------------------------------------
+     TODO: - check if theses "set_expression" will ever produce stmts as well, otherwise remove from here
+           - replace concatination in the return with a general function
+-------------------------------------------------*)
+Definition compile_table_variables_def:
+  compile_table_variables env [] = return (env, [], []) ∧
+  compile_table_variables env (((ss, p), a)::tbls) =
   do
-    (env', x) <<- generate_varname env;
-    v_l1::v_ls <<- lCOPY prms;
-    (env'', s_l1::s_ls) <- FOLDL (\(e, x_p) x. let (e', x_p') = compile_exp e x in (e', x_p::x_p') ) (env', []) sls;
-    
-    s <<- DecCall x One env.match_fun [v_l1]::[s_l1] Skip;
-    prog <<- FOLDL ((\env prev v. let (env', r) = generate_varname env
-                                       in (x, Seq s $ DecCall r One env.match_fun v_l::s_l $ Assign Local x (Op And [r]::[x])))) env'') (x, s) ZIP (v_ls, s_ls);
-    return (env'', x, prog)
+    (env', stmts, es_pan) <- compile_set_exp env ss;
+    (env'', stmts', l)   <- compile_table_variables env' tbls;
+    return (env'', (stmts++stmts'), l++[((es_pan, p), a)])
   od
 End
         
-(*
-Ebpf-architecture specific table matching function (as of yet).
-*)
+(*-------------------------------------------------
+ASSUMTIONS: - priority in tbl for certain action is of type bit-string
+      TODO: - fun_end need real return value
+            - only Ebpf-architecture specific
+            - what to do with params?
+-------------------------------------------------*)
 Definition compile_action_tables_def:
-  compile_action_tables env vars [] = return (env, []) ∧
-  compile_action_tables env vars (table_name, (mks, (default_action, es)))::ts =
+  compile_action_tables env [] = return (env, []) ∧
+  compile_action_tables env ((table_name, (mks, (default_action, es)))::ts) =
   do
-    (env', prms) <- FOLDL (\(e, x_p) x. let (e', x_p') = compile_exp e x in (e', x_p::x_p') ) (env, []) es;
-    b <<- Skip;
-
-    case env.tbl of
-      tbls =>
-        do
-          (env'', action) <<- generate_varname env';
-          (env''', priority) <<- generate_varname env'';
-          (env4, found) <<- generate_varname env''';
-                 
-          s <<- Dec action One (Const w0 :64 word) $ Dec priority One (Const w0 :64 word) $ Dec found One (Const w0 :64 word) Skip;
-          fun_end <<- Return TopAddr; (* TODO *)
-          tbls' <- FOLDR ((\(e, prev) ((s, p), a). do (e', s'); return ((s',p),a)::prev) env) [] tbls;
-          (env5, prog) <<- FOLDL((\v_ls (e, prev) action priority found ((s_ls, prio), a).
-                                    (let
-                                       (e', x, p_a) = generate_action_matching e v_ls s_ls;
-                                       ass_a    = Assign Local action a;
-                                       ass_prio = Assign Local priority prio;
-                                       p_true   = If (Op (Cmp lower) [priority]::[prio]) (Seq ass_a ass_prio) (Skip);
-                                       p_false  = Seq ass_a ass_prio;
-                                       p_true'  = If found p_true p_false;
-                                       p_false' = Skip;
-                                       p_conds  = Seq (If x p_true' p_false') (Skip);
-                                     in
-                                       (e', Seq (Seq p_a p_conds) prev))) v_ls action priority found) (env4, fun_end) tbls';      
-          b <<- prog)
-        od
-    | [] =>)
+    (env', stmts, args :64 exp list) <- compile_exps env es;
+    (env'', fun_prms) <<- generate_params env' args;
+    tbl <<- env''.table;
+    (env''', a_s) <<- generate_varname env'';
+    (env4, p_s)   <<- generate_varname env''';
+    (env5, f_s)   <<- generate_varname env4;
+    found   <<- Var Local f_s;
+    (env6, stmts, tbl') <- compile_table_variables env5 tbl;
+    start_prog <<- (Dec a_s One (Const (0w :64 word)) $ Dec p_s One (Const (0w :64 word)) $ Dec f_s One (Const (0w :64 word)) Skip);
+    pre_prog   <<- to_seq stmts;
+    (env7, prog) <<- generate_actions env6 (args, a_s, p_s, found) tbl';
     decl <<-
-         <|       name   := get_fun_name n
-                ; inline := F
-                ; export := F
-                ; params := prms
-                ; body   := b
-                ; return := One
+         <|         name   := strlit (get_fun_name table_name)
+                  ; inline := F
+                  ; export := F
+                  ; params := fun_prms
+                  ; body   := Seq (Seq start_prog pre_prog) prog
+                  ; return := One
          |>;
+    (env8, decls) <- compile_action_tables env7 ts;
+    return (env8, decl::decls)
   od
 End
 
+(*-------------------------------------------------
+
+-------------------------------------------------*)
 Definition compile_control_def:
   compile_control env n b_func_map func_map sd_list tbl_map t_scope =
      do
-       vars <<- get_local_vars t_scope;
+       vars <<- get_local_vars t_scope;                                       (* TODO: this only gives names, not expressions *)
        prms <<- to_params sd_list;
        (env', decls) <- compile_block_functions env vars b_func_map;          (*important to be before block compilation (dir. depend on stmt-compilation order)*)
-       (env'', table_decls) <- compile_action_tables env' vars tbl_map;
+       (env'', table_decls) <- compile_action_tables env' tbl_map;
        b <- lookup_block_body n b_func_map;
        (env''', b') <- compile_stmt env' b;
        cntrl_decl <<-
@@ -437,9 +591,13 @@ Definition compile_control_def:
              ; body   := b' 
              ; return := One
        |>;
-       return (env''', decls::(table_decl::cntrl_decl))
+       d <<- table_decls++[cntrl_decl];
+       return (env''', decls++d)
      od
 End
+
+
+
 
 (*
 -------------------------------------------------
@@ -506,30 +664,30 @@ Definition compile_archblocks_def:
 End
         
 Definition compile_global_funs_def:
-  compile_global_funs env [] = return (env, [])
-  compile_global_funs env (s, (stmt, sd_list))::func_map =
+  compile_global_funs env [] = return (env, []) ∧
+  compile_global_funs env ((s, (stmt, sd_list))::func_map) =
   do
-    (env', body_pan) <- compile_stmt stmt env ;
+    (env', body_pan) <- compile_stmt env stmt;
     prms <<- to_params sd_list;
     decl <<-
-    <|         name        := get_fun_name s
+    <|         name        := (strlit (get_fun_name s))
              ; inline      := F
              ; export      := F
              ; params      := prms
              ; body        := body_pan
              ; return      := One
-    |> :64 fun_decl;
+    |>;
     (env'', decls) <- compile_global_funs env' func_map;
-    return (env'', decl::decls))
+    return (env'', decl::decls)
   od
 End
 
 Definition compile_actx_def:
   compile_actx env (abs, (_, pblock_ms), _, _, _, _, _, apply_table, _, func_map) =
   do
-    (env', global_decls) <- compile_global_funs func_map;
+    (env', global_decls) <- compile_global_funs env func_map;
     (env'', decls) <- compile_archblocks env' pblock_ms abs func_map;
-    return decls::global_decls
+    return (decls++global_decls)
   od
 End
 
@@ -538,13 +696,15 @@ End
 (*                    SETUP                        *)
 (*-------------------------------------------------*)
 Definition env_setup_def:
-  env_setup ((_, _, _, tbl), _, _, _) =
+  env_setup ((_, _, _, tbl :ebpf_ctrl), _, _, _) =
   (let
     dict1 = FEMPTY : word64 state_dict;
     dict2 = FEMPTY : scope_dict;
     dict3 = FEMPTY : staten_dict;
-    dict4 = FEMPTY : word64 out_ind_dict;
-    env = <| states := dict1 ; scopes := dict2 ; state_nums := dict3 ; out_ind := dict4 ; table := tbl |>;
+    dict4 = FEMPTY : out_ind_dict;
+    dict5 = FEMPTY : out_val_dict;
+    pvar = varn_name "";
+    env = <| states := dict1 ; scopes := dict2 ; state_nums := dict3 ; out_s_ind_pairs := dict4 ; table := tbl ; ass_var := pvar ; out_ind_val_pairs := dict5 ; match_fun := get_match_fun_name |>;
    in
      return env)
 End
@@ -555,7 +715,7 @@ End
 
 (*
    For now, aenv is assumed to have 'a <- ebpf_scope, thus is only for the ebpf architecture.
-*)
+*)(*
 Definition compile_def:
   compile_def actx (aenv, _, _, _) =
   do
@@ -566,4 +726,4 @@ Definition compile_def:
     | SOME => NONE (*some_pancake_function pancake_program*)
   od
 End
-
+*)
